Prove invariance of graph semantics under edge order (assuming tensors are permutative)

theories/GraphCore/TensorGraphExpr.v
@@ -2,6 +2,20 @@ Require Export TensorGraph Aux_pos.
 
 Require Export TensorExprDBSyntax.
 
+(* FIXME: Move: *)
+Require Combinators.
+
+(* FIXME: Move: *)
+Lemma pseq_to_seq_inv (start len : nat) :
+  Pos.of_succ_nat <$> seq start len =
+  pseq (Pos.of_succ_nat start) (N.of_nat len).
+Proof.
+  rewrite pseq_to_seq.
+  do 2 f_equal; lia.
+Qed.
+
+#[local] Coercion pos_to_nat_pred : positive >-> nat.
+
 (* Semantics of TensorGraphs into tensor expressions *)
 
 
@@ -13,18 +27,18 @@ Let TensorGraph := (TensorGraph T).
 
 Implicit Types tg : TensorGraph.
 
-Definition input_edges (linternal lexternal : list labedge) 
+Definition input_edges (linternal lexternal : list labedge)
   (k : nat) : list var :=
-  ((rel ∘ Pos.of_succ_nat ∘ fst) <$> 
+  ((rel ∘ Pos.of_succ_nat ∘ fst) <$>
     node_input_edges k linternal) ++
-  ((loc ∘ bcons false ∘ Pos.of_succ_nat ∘ fst) <$> 
+  ((loc ∘ bcons false ∘ Pos.of_succ_nat ∘ fst ∘ snd) <$>
     node_input_edges k lexternal).
 
-Definition output_edges (linternal lexternal : list labedge) 
+Definition output_edges (linternal lexternal : list labedge)
   (k : nat) : list var :=
-  ((rel ∘ Pos.of_succ_nat ∘ fst) <$> 
+  ((rel ∘ Pos.of_succ_nat ∘ fst) <$>
     node_output_edges k linternal) ++
-  ((loc ∘ bcons false ∘ Pos.of_succ_nat ∘ fst) <$> 
+  ((loc ∘ bcons true ∘ Pos.of_succ_nat ∘ snd ∘ snd) <$>
     node_output_edges k lexternal).
 
 
@@ -39,7 +53,991 @@ Definition mk_node (linternal lexternal : list labedge)
 
 Definition graph_tensorlist_semantics (tg : TensorGraph) : tensorlist :=
   mk_tl (const 0%nat <$> internal_edges tg)
-    (mk_node (i_internal_edges tg) (i_external_edges tg) <$> 
+    (mk_node (i_internal_edges tg) (i_external_edges tg) <$>
       (map_to_list (fst tg)).*1).
+
+Definition num_internals (tg : TensorGraph) : nat :=
+  length (internal_edges tg).
+
+Definition num_externals (tg : TensorGraph) : nat :=
+  length (external_edges tg).
+
+#[global] Arguments num_internals !_ /.
+#[global] Arguments num_externals !_ /.
+
+Definition graph_namedtensorlist_semantics_aux
+  (lint lext : list labedge) (ks : list nat) :=
+  mk_ntl ((., O) ∘ Pos.of_succ_nat ∘ fst <$>
+    lint)
+    (mk_node lint
+      lext <$>
+      ks).
+
+Definition graph_namedtensorlist_semantics (tg : TensorGraph)
+  (int_labs ext_labs : list nat) : namedtensorlist :=
+  mk_ntl (zip_with (λ i _, (Pos.of_succ_nat i, O)) int_labs $ internal_edges tg)
+    (mk_node (zip int_labs (internal_edges tg))
+      (zip ext_labs (external_edges tg)) <$>
+      (map_to_list (nodes tg)).*1).
+
+Lemma graph_namedtensorlist_semantics_to_aux tg int_labs ext_labs :
+  graph_namedtensorlist_semantics tg int_labs ext_labs =
+  graph_namedtensorlist_semantics_aux
+    (zip int_labs (internal_edges tg)) (zip ext_labs (external_edges tg))
+    (map_to_list (nodes tg)).*1.
+Proof.
+  unfold graph_namedtensorlist_semantics, graph_namedtensorlist_semantics_aux.
+  rewrite fmap_zip_with.
+  reflexivity.
+Qed.
+
+
+Definition graph_tabst (tg : TensorGraph) : Pmap (nat * nat) :=
+  kmap Pos.of_succ_nat $
+  map_imap (λ (k : nat) (_ : T), Some (length (filter (is_node_input k) (edges tg)),
+    length (filter (is_node_output k) (edges tg)))) (nodes tg).
+
+
+Lemma fold_internal_edges tg :
+  filter (is_internal (nodes tg)) (edges tg) = internal_edges tg.
+Proof. reflexivity. Qed.
+
+Lemma fold_external_edges tg :
+  filter (not_internal (nodes tg)) (edges tg) = external_edges tg.
+Proof. reflexivity. Qed.
+
+Lemma fold_num_internals tg :
+  length (internal_edges tg) = num_internals tg.
+Proof. reflexivity. Qed.
+
+Lemma fold_num_externals tg :
+  length (external_edges tg) = num_externals tg.
+Proof. reflexivity. Qed.
+
+Lemma graph_namedtensorlist_semantics_seq_correct tg :
+  graph_namedtensorlist_semantics tg (seq 0 (num_internals tg))
+    (seq 0 (num_externals tg)) = tl2ntl (graph_tensorlist_semantics tg).
+Proof.
+  cbn -[reverse].
+  rewrite fmap_const, reverse_replicate.
+  rewrite fold_internal_edges; fold (num_internals tg) (num_externals tg).
+  rewrite fold_external_edges.
+  unfold graph_namedtensorlist_semantics.
+  f_equal.
+  - rewrite imap_to_zip_with_seq, length_replicate.
+    unfold num_internals.
+    rewrite <- fmap_const, zip_with_fmap_r.
+    reflexivity.
+  - now rewrite 2 imap_to_zip_with_seq.
+Qed.
+
+Lemma list_fmap_subseteq {A B} (f : A -> B) (l1 l2 : list A) :
+  l1 ⊆ l2 -> f <$> l1 ⊆ f <$> l2.
+Proof.
+  intros Hl b (a & -> & ?%Hl)%elem_of_list_fmap.
+  now apply elem_of_list_fmap_1.
+Qed.
+
+Lemma list_subseteq_app {A} {l1 l1' l2 l2' : list A} :
+  l1 ⊆ l1' -> l2 ⊆ l2' -> l1 ++ l2 ⊆ l1' ++ l2'.
+Proof.
+  intros;
+  apply list_subseteq_app_iff_l, conj;
+    [apply list_subseteq_app_l|apply list_subseteq_app_r];
+  done.
+Qed.
+
+Lemma input_edges_subseteq_labels lint lext k :
+  input_edges lint lext k ⊆
+    (rel ∘ Pos.of_succ_nat ∘ fst <$> lint) ++
+    (loc ∘ bcons false ∘ Pos.of_succ_nat ∘ fst ∘ snd <$> lext).
+Proof.
+  unfold input_edges.
+  apply list_subseteq_app;
+  apply list_fmap_subseteq, list_filter_subseteq.
+Qed.
+
+Lemma output_edges_subseteq_labels lint lext k :
+  output_edges lint lext k ⊆
+    (rel ∘ Pos.of_succ_nat ∘ fst <$> lint) ++
+    (loc ∘ bcons true ∘ Pos.of_succ_nat ∘ snd ∘ snd <$> lext).
+Proof.
+  unfold output_edges.
+  apply list_subseteq_app;
+  apply list_fmap_subseteq, list_filter_subseteq.
+Qed.
+
+
+Lemma graph_tensorlist_semantics_WF tg :
+  WF_tl (graph_tensorlist_semantics tg).
+Proof.
+  intros i.
+  rewrite elem_of_abstracts_rel_vars.
+  cbn -[internal_edges external_edges].
+  rewrite length_fmap, fold_num_internals.
+  intros (f & low & up & (k & [= -> -> ->] & Hk)%elem_of_list_fmap & Hi).
+  apply (elem_of_list_to_set (C:=gset nat)) in Hk.
+  rewrite <- dom_alt in Hk.
+  apply (list_subseteq_app (input_edges_subseteq_labels _ _ _)
+    (output_edges_subseteq_labels _ _ _)) in Hi.
+  rewrite Permutation_swap_app_app, elem_of_app in Hi.
+  destruct Hi as [Hi|HF]. 2:{
+    rewrite !Combinators.compose_assoc in HF.
+    rewrite 2 (list_fmap_compose _ loc), <- fmap_app in HF.
+    apply elem_of_list_fmap in HF as (? & [=] & _).
+  }
+  revert Hi.
+  rewrite elem_of_app, (or_idemp _).
+  rewrite Combinators.compose_assoc, list_fmap_compose.
+  rewrite elem_of_list_fmap_inj by apply _.
+  unfold i_internal_edges, enumerate.
+  rewrite fmap_imap.
+  unfold compose; cbn -[internal_edges].
+  rewrite imap_seq_0, pseq_to_seq_inv.
+  intros ?%elem_of_pseq_1.
+  rewrite fold_num_internals in Hi.
+  lia.
+Qed.
+
+Lemma uncurry_alt {A B C} (f : A -> B -> C) p :
+  uncurry f p = f p.1 p.2.
+Proof.
+  now destruct p.
+Qed.
+
+Lemma graph_namedtensorlist_semantics_WF tg int_lab ext_lab :
+  NoDup int_lab -> length int_lab = num_internals tg ->
+  WF_ntl (graph_namedtensorlist_semantics tg int_lab ext_lab).
+Proof.
+  intros Hdupi Hleni.
+  split.
+  - cbn.
+    rewrite zip_with_zip.
+    erewrite (list_fmap_ext (uncurry _ )) by now intros; rewrite uncurry_alt.
+    rewrite <- list_fmap_compose.
+    unfold compose; cbn.
+    setoid_rewrite (list_fmap_compose fst Pos.of_succ_nat).
+    rewrite fst_zip by now apply eq_reflexivity.
+    apply NoDup_fmap_2; [apply _|done].
+  - intros r.
+    rewrite elem_of_abstracts_rel_vars, elem_of_list_to_set.
+    cbn -[internal_edges external_edges].
+    intros (f & low & up & (k & [= -> -> ->] & Hk)%elem_of_list_fmap & Hi).
+    apply (elem_of_list_to_set (C:=gset nat)) in Hk.
+    rewrite <- dom_alt in Hk.
+    apply (list_subseteq_app (input_edges_subseteq_labels _ _ _)
+      (output_edges_subseteq_labels _ _ _)) in Hi.
+    rewrite Permutation_swap_app_app, elem_of_app in Hi.
+    destruct Hi as [Hi|HF]. 2:{
+      rewrite !Combinators.compose_assoc in HF.
+      rewrite 2 (list_fmap_compose _ loc), <- fmap_app in HF.
+      apply elem_of_list_fmap in HF as (? & [=] & _).
+    }
+    revert Hi.
+    rewrite elem_of_app, (or_idemp _).
+    rewrite Combinators.compose_assoc, list_fmap_compose.
+    rewrite elem_of_list_fmap_inj by apply _.
+    unfold i_internal_edges, enumerate.
+    rewrite 2 fmap_zip_with.
+    easy.
+Qed.
+
+Lemma relabel_rels_node_input_edges lint k fint :
+  prod_map fint id <$>
+    (node_input_edges k lint) =
+  node_input_edges k (prod_map fint id <$> lint).
+Proof.
+  unfold node_input_edges.
+  rewrite list_filter_fmap.
+  reflexivity.
+Qed.
+
+Lemma relabel_rels_node_output_edges lext k fint :
+  prod_map fint id <$>
+    (node_output_edges k lext) =
+  node_output_edges k (prod_map fint id <$> lext).
+Proof.
+  unfold node_output_edges.
+  rewrite list_filter_fmap.
+  reflexivity.
+Qed.
+
+Lemma relabel_rels_input_edges lint lext k fint :
+  relabel_rels (Pos.of_succ_nat ∘ fint ∘ pos_to_nat_pred) <$>
+    (input_edges lint lext k) =
+  input_edges (prod_map fint id <$> lint) lext k.
+Proof.
+  unfold input_edges.
+  rewrite <- relabel_rels_node_input_edges.
+  rewrite <- list_fmap_compose, fmap_app, <- !list_fmap_compose.
+  f_equal.
+  now apply list_fmap_ext; intros _ ? _; cbn; rewrite pos_to_nat_pred_of_nat.
+Qed.
+
+Lemma relabel_rels_output_edges lint lext k fint :
+  relabel_rels (Pos.of_succ_nat ∘ fint ∘ pos_to_nat_pred) <$>
+    (output_edges lint lext k) =
+  output_edges (prod_map fint id <$> lint) lext k.
+Proof.
+  unfold output_edges.
+  rewrite <- relabel_rels_node_output_edges.
+  rewrite <- list_fmap_compose, fmap_app, <- !list_fmap_compose.
+  f_equal.
+  now apply list_fmap_ext; intros _ ? _; cbn; rewrite pos_to_nat_pred_of_nat.
+Qed.
+
+
+Lemma relabel_rels_mk_node lint lext k fint :
+  relabel_abs (relabel_rels (Pos.of_succ_nat ∘ fint ∘ pos_to_nat_pred))
+    (mk_node lint lext k) =
+  mk_node (prod_map fint id <$> lint) lext k.
+Proof.
+  unfold mk_node; cbn.
+  now rewrite relabel_rels_input_edges, relabel_rels_output_edges.
+Qed.
+
+
+Lemma relabel_rels_input_edges' lint lext k fr :
+  relabel_rels fr <$>
+    (input_edges lint lext k) =
+  input_edges (prod_map (pos_to_nat_pred ∘ fr ∘ Pos.of_succ_nat) id <$> lint) lext k.
+Proof.
+  rewrite <- relabel_rels_input_edges.
+  apply list_fmap_ext; intros _ ? _; apply relabel_rels_ext; intros ?;
+  unfold compose; cbn; now rewrite !pos_to_nat_pred_to_pos.
+Qed.
+
+Lemma relabel_rels_output_edges' lint lext k fr :
+  relabel_rels fr <$>
+    (output_edges lint lext k) =
+  output_edges (prod_map (pos_to_nat_pred ∘ fr ∘ Pos.of_succ_nat) id <$> lint) lext k.
+Proof.
+  rewrite <- relabel_rels_output_edges.
+  apply list_fmap_ext; intros _ ? _; apply relabel_rels_ext; intros ?;
+  unfold compose; cbn; now rewrite !pos_to_nat_pred_to_pos.
+Qed.
+
+Lemma relabel_rels_mk_node' lint lext k fr :
+  relabel_abs (relabel_rels fr)
+    (mk_node lint lext k) =
+  mk_node (prod_map (pos_to_nat_pred ∘ fr ∘ Pos.of_succ_nat) id <$> lint) lext k.
+Proof.
+  unfold mk_node; cbn.
+  now rewrite relabel_rels_input_edges', relabel_rels_output_edges'.
+Qed.
+
+
+
+Lemma graph_namedtensorlist_semantics_reindex_int
+  (fint : nat -> nat) `{Hfint : !Inj eq eq fint} tg int_lab ext_lab :
+  graph_namedtensorlist_semantics tg (fint <$> int_lab) ext_lab =ntl=
+  graph_namedtensorlist_semantics tg int_lab ext_lab.
+Proof.
+  (* intros Hdupi Hleni. *)
+  symmetry.
+  hnf.
+  exists (Pos.of_succ_nat ∘ fint ∘ pos_to_nat_pred).
+  split; [intros ????; apply (inj _)|].
+  split.
+  - cbn -[internal_edges].
+    rewrite fmap_zip_with, zip_with_fmap_l.
+    cbn.
+    apply eq_reflexivity, zip_with_ext; now intros;
+    rewrite ?pos_to_nat_pred_of_nat.
+  - cbn -[internal_edges external_edges].
+    apply eq_reflexivity.
+    rewrite <- list_fmap_compose.
+    apply list_fmap_ext; intros _ k _.
+    unfold compose at 1.
+    rewrite relabel_rels_mk_node.
+    now rewrite fmap_zip_with, zip_with_fmap_l.
+Qed.
+
+Arguments internal_edges !_ /.
+Arguments external_edges !_ /.
+
+Lemma internal_external_decomp tg :
+  edges tg ≡ₚ internal_edges tg ++ external_edges tg.
+Proof.
+  unfold internal_edges, external_edges.
+  symmetry.
+  apply filter_with_neg_Permutation.
+Qed.
+
+Lemma mk_node_abst_WT'_aux tg int_lab ext_lab k :
+  (num_internals tg <= length int_lab)%nat ->
+  (num_externals tg <= length ext_lab)%nat ->
+  k ∈ dom (nodes tg) ->
+  abst_WT' (graph_tabst tg)
+    (mk_node (zip int_lab (internal_edges tg)) (zip ext_lab (external_edges tg))
+      k).
+Proof.
+  intros Hilab Helab Hk.
+  unfold abst_WT';
+  cbn.
+  unfold graph_tabst.
+  rewrite lookup_kmap by apply _.
+  rewrite map_lookup_imap.
+  apply elem_of_dom in Hk as [t Ht].
+  rewrite Ht.
+  cbn.
+  f_equal.
+  rewrite internal_external_decomp, 2 filter_app.
+  unfold input_edges, output_edges.
+  rewrite !length_app, ! length_fmap.
+  rewrite <- ! length_app.
+  unfold node_input_edges, node_output_edges.
+  rewrite <- 4 filter_app.
+  f_equal; symmetry;
+  rewrite <- (length_fmap snd), <- list_filter_fmap, fmap_app, 2 snd_zip by easy;
+  reflexivity.
+Qed.
+
+
+Lemma mk_node_abst_WT'_imap_pair tg k :
+  k ∈ dom (nodes tg) ->
+  abst_WT' (graph_tabst tg)
+    (mk_node (imap pair (internal_edges tg)) 
+      (imap pair (external_edges tg))
+      k).
+Proof.
+  intros Hk.
+  rewrite 2 imap_to_zip_with_seq.
+  apply mk_node_abst_WT'_aux; now try rewrite length_seq.
+Qed.
+
+Import SetoidList SetoidPermutation list.
+
+
+Lemma input_edges_perm_eq lint lint' lext lext' k :
+  lint ≡ₚ lint' -> lext ≡ₚ lext' ->
+  input_edges lint lext k ≡ₚ input_edges lint' lext' k.
+Proof.
+  intros Hlint Hlext.
+  unfold input_edges.
+  do 2 f_equiv;
+  unfold node_input_edges;
+  now f_equiv.
+Qed.
+
+Lemma output_edges_perm_eq lint lint' lext lext' k :
+  lint ≡ₚ lint' -> lext ≡ₚ lext' ->
+  output_edges lint lext k ≡ₚ output_edges lint' lext' k.
+Proof.
+  intros Hlint Hlext.
+  unfold output_edges.
+  do 2 f_equiv;
+  unfold node_output_edges;
+  now f_equiv.
+Qed.
+
+Lemma mk_node_perm_eq lint lint' lext lext' k :
+  lint ≡ₚ lint' -> lext ≡ₚ lext' ->
+  mk_node lint lext k ≡abs≡ₚ mk_node lint' lext' k.
+Proof.
+  intros Hlint Hext.
+  unfold mk_node; cbn.
+  split_and!; cbn;
+  [done|now apply input_edges_perm_eq|now apply output_edges_perm_eq].
+Qed.
+
+(* FIXME: Move *)
+Lemma zip_Permutation_l_exists_r {A B} (l l' : list A) (k : list B) :
+  l ≡ₚ l' ->
+  length l = length k ->
+  exists k', k ≡ₚ k' /\
+  zip l k ≡ₚ zip l' k'.
+Proof.
+  intros Hl.
+  revert k;
+  induction Hl; intros k.
+  - destruct k; [|done].
+    now exists [].
+  - destruct k as [|y k]; [done|].
+    intros [= (k' & Hk & Hzip)%IHHl].
+    exists (y :: k').
+    split; now cbn; f_equiv.
+  - destruct k as [|y' [|x' k]]; [done..|].
+    intros _.
+    exists (x' :: y' :: k).
+    split; cbn; solve_Permutation.
+  - intros Hlen.
+    apply IHHl1 in Hlen as Hk'.
+    destruct Hk' as (k' & Hkk' & Hzip).
+    pose proof Hlen as Hlen'.
+    rewrite Hl1, Hkk' in Hlen'.
+    apply IHHl2 in Hlen' as (k'' & Hk'k'' & Hzip').
+    exists k''.
+    split; solve [eauto using Permutation_trans].
+Qed.
+Lemma zip_Permutation_r_exists_l {A B} (l : list A) (k k' : list B) :
+  k ≡ₚ k' ->
+  length l = length k ->
+  exists l', l ≡ₚ l' /\
+  zip l k ≡ₚ zip l' k'.
+Proof.
+  intros Hk Hlen%eq_sym.
+  destruct (zip_Permutation_l_exists_r k k' l Hk Hlen) as (l' & Hl' & Hzip).
+  exists l'.
+  split; [easy|].
+  rewrite <- 2 (@zip_with_flip A B).
+  apply (fmap_Permutation prod_swap) in Hzip.
+  rewrite 2 fmap_zip_with in Hzip.
+  apply Hzip.
+Qed.
+
+
+
+
+(*
+Lemma input_edges_edges_perm_eq int_lab ints ints'
+  ext_lab exts exts' k :
+  ints ≡ₚ ints' -> exts ≡ₚ exts' ->
+  length int_lab = length ints ->
+  length ext_lab = length exts ->
+  input_edges (zip int_lab ints) (zip ext_lab exts) k ≡ₚ
+  input_edges (zip int_lab ints') (zip ext_lab exts') k.
+Proof.
+  intros Hints Hexts Hleni Hlene.
+  unfold input_edges.
+  f_equiv.
+  - rewrite 2 (list_fmap_compose fst).
+    unfold node_input_edges.
+    rewrite list_filter_fmap.
+    rewrite <- Combinators.compose_assoc.
+  intros Hlint Hlext Hleni Hlene.
+  specialize
+  unfold input_edges.
+  do 2 f_equiv;
+  unfold node_input_edges;
+  now f_equiv.
+Qed. *)
+
+(* Lemma input_edges_lab_perm_eq int_lab int_lab' ints
+  ext_lab ext_lab' exts k :
+  int_lab ≡ₚ int_lab' -> ext_lab ≡ₚ ext_lab' ->
+  length int_lab = length ints ->
+  length ext_lab = length exts ->
+  input_edges (zip int_lab ints) (zip ext_lab exts) k ≡ₚ
+  input_edges (zip int_lab' ints) (zip ext_lab' exts) k.
+Proof.
+  intros Hlint Hlext Hleni Hlene.
+  specialize
+  unfold input_edges.
+  do 2 f_equiv;
+  unfold node_input_edges;
+  now f_equiv.
+Qed. *)
+
+
+Lemma graph_namedtensorlist_semantics_aux_perm_eq' lint lint' lext lext' ks ks' :
+  NoDup lint.*1 -> lint ≡ₚ lint' ->
+  lext ≡ₚ lext' -> ks ≡ₚ ks' ->
+  graph_namedtensorlist_semantics_aux lint lext ks ≡ntl'≡ₚ
+  graph_namedtensorlist_semantics_aux lint' lext' ks'.
+Proof.
+  intros Hdup Hlint Hlext Hks.
+  split; cbn.
+  - apply list_to_map_proper; [|now f_equiv].
+    rewrite <- list_fmap_compose.
+    unfold compose; cbn.
+    change (_ <$> _) with (Pos.of_succ_nat ∘ fst <$> lint).
+    rewrite list_fmap_compose.
+    now apply (NoDup_fmap_2 _ _).
+  - etransitivity; [|apply (Permutation_PermutationA _); now rewrite <- Hks].
+    apply eqlistA_PermutationA.
+    apply eqlistA_altdef.
+    rewrite Forall2_fmap.
+    apply Forall_Forall2_diag, (set_Forall_list_to_set (C:=gset nat)).
+    intros k _.
+    now apply mk_node_perm_eq.
+Qed.
+
+(* FIXME: Move *)
+Lemma ntl_aeq_WF ntl ntl' :
+  ntl =ntl= ntl' -> WF_ntl ntl -> WF_ntl ntl'.
+Proof.
+  intros (fr & Hfr & Hfsums & Hfabs).
+  cbn.
+  intros [Hdup Habs].
+  split.
+  - rewrite <- Hfsums.
+    rewrite fsts_prod_map.
+    apply NoDup_fmap_2_strong, Hdup.
+    intros ? ? Hx Hy; apply Hfr; set_solver + Hx Hy.
+  - rewrite <- Hfsums, <- Hfabs.
+    rewrite abstracts_rel_vars_relabel_rels, fsts_prod_map,
+      <- (set_map_list_to_set_L (SA:=Pset)).
+    f_equiv; apply Habs.
+Qed.
+Lemma ntl_aeq_of_WF ntl ntl' : WF_ntl ntl ->
+  (exists fr,
+    set_Forall2 (λ i j, fr i = fr j -> i = j) (list_to_set ntl.(ntl_sums).*1:>Pset ) /\
+    prod_map fr id <$> ntl.(ntl_sums) ≡ₚ ntl'.(ntl_sums) /\
+    relabel_abs (relabel_rels fr) <$> ntl.(ntl_abstracts) ≡ₚ ntl'.(ntl_abstracts)
+    ) ->
+  ntl =ntl= ntl'.
+Proof.
+  intros HWF (fr & Hfr & Hsums & Habs).
+  exists fr.
+  split; [|easy].
+  intros x y Hx Hy.
+  apply Hfr; specialize (HWF.2); [set_solver +Hx|set_solver +Hy].
+Qed.
+
+(* FIXME: Move *)
+Section list_index.
+Context `{EqDecision A}.
+Implicit Type l : list A.
+
+Definition list_index (x : A) l :=
+  fst <$> list_find (eq x) l.
+
+Lemma list_index_is_Some x l :
+  is_Some (list_index x l) <-> x ∈ l.
+Proof.
+  unfold list_index.
+  rewrite fmap_is_Some.
+  split; [|intros Hx; apply (list_find_elem_of _ _ x Hx eq_refl)].
+  now intros [[] (?%elem_of_list_lookup_2 & <- & _)%list_find_Some].
+Qed.
+
+Lemma list_index_Some x l i :
+  list_index x l = Some i <->
+  l !! i = Some x /\ forall j y, l !! j = Some y -> j < i -> x <> y.
+Proof.
+  unfold list_index.
+  rewrite fmap_Some, exists_pair.
+  setoid_rewrite list_find_Some.
+  naive_solver.
+Qed.
+
+Lemma list_index_Some_NoDup x l i :
+  NoDup l ->
+  list_index x l = Some i <-> l !! i = Some x.
+Proof.
+  intros Hdup.
+  rewrite list_index_Some.
+  rewrite <- (and_True (l !! i = Some x)) at 2.
+  apply and_iff_from_l; [reflexivity|intros Hli _].
+  apply iff_True_1.
+  intros j y Hlj Hji ->.
+  enough (i = j) by lia.
+  revert Hli Hlj.
+  now apply NoDup_lookup.
+Qed.
+
+Lemma list_index_inj x y l i :
+  list_index x l = Some i -> list_index y l = Some i -> x = y.
+Proof.
+  rewrite 2 list_index_Some.
+  intros [] [].
+  congruence.
+Qed.
+
+Lemma list_index_lt x l i :
+  list_index x l = Some i -> i < length l.
+Proof.
+  now intros [?%lookup_lt_Some _]%list_index_Some.
+Qed.
+
+Lemma list_index_ppermute_NoDup x l f : posperm (lengthP l) f ->
+  NoDup l ->
+  list_index x (ppermute f l) =
+  (pos_to_nat_pred ∘ posperm_inv (lengthP l) f ∘ Pos.of_succ_nat) <$> list_index x l.
+Proof.
+  intros Hf Hl.
+  apply option_eq; intros i.
+  rewrite list_index_Some_NoDup by now rewrite ppermute_permutation.
+  pose proof (lengthN_correct l).
+  split.
+  - intros Hlook.
+    apply lookup_lt_Some in Hlook as Hi.
+    rewrite length_ppermute in Hi.
+    rewrite lookup_ppermute_alt_bdd in Hlook by now easy + apply posperm_bounded.
+    replace (list_index x l) with (Some (f (Pos.of_succ_nat i) :> nat)) by
+      now symmetry; apply list_index_Some_NoDup.
+    cbn.
+    rewrite pos_to_nat_pred_to_pos.
+    rewrite posperm_inv_linv by now easy + lia.
+    f_equal; lia.
+  - destruct (list_index x l) as [fi|] eqn:Hfi; [|easy].
+    apply list_index_Some in Hfi as [Hfi _].
+    apply lookup_lt_Some in Hfi as Hfilt.
+    cbn.
+    intros [= <-].
+    rewrite lookup_ppermute_alt_bdd by first [
+      now apply posperm_bounded|
+      specialize (posperm_inv_bounded (lengthP l) f (Pos.of_succ_nat fi));
+      lia
+    ].
+    rewrite pos_to_nat_pred_to_pos.
+    rewrite posperm_inv_rinv by now easy || lia.
+    now rewrite pos_to_nat_pred_of_nat.
+Qed.
+
+Lemma list_lookup_omap_all_is_Some `(f : A -> option B) (l : list A) (i : nat)
+  (Hf : forall a, a ∈ l -> is_Some (f a)) :
+  omap f l !! i = l !! i ≫= f.
+Proof.
+  rewrite <- Forall_forall in Hf.
+  revert i;
+  induction Hf; [now intros []|intros i].
+  cbn.
+  destruct (f x) as [fx|] eqn:Hfx; [|now rewrite is_Some_alt in *].
+  destruct i; [cbn; now rewrite Hfx|].
+  cbn.
+  apply IHHf.
+Qed.
+
+Lemma length_omap_all_is_Some `(f : A -> option B) (l : list A)
+  (Hf : forall a, a ∈ l -> is_Some (f a)) :
+  length (omap f l) = length l.
+Proof.
+  rewrite <- Forall_forall in Hf.
+  induction Hf; [done|cbn].
+  destruct (f x) as [fx|] eqn:Hfx; [|now rewrite is_Some_alt in *].
+  cbn.
+  f_equal; apply IHHf.
+Qed.
+
+Lemma omap_all_is_Some_default `(f : A -> option B) (l : list A) (g : A -> B)
+  (Hf : forall a, a ∈ l -> is_Some (f a)) :
+  omap f l = (λ i, default (g i) (f i)) <$> l.
+Proof.
+  apply (list_eq_same_length _ _ _ eq_refl).
+  - now rewrite length_fmap; apply length_omap_all_is_Some.
+  - intros i x y.
+    rewrite length_fmap.
+    intros Hi.
+    rewrite list_lookup_omap_all_is_Some by easy.
+    rewrite list_lookup_fmap.
+    destruct (l !! i) as [li|]; [|easy].
+    cbn.
+    destruct (f li); [|easy].
+    cbn; congruence.
+Qed.
+
+Lemma ppermute_alt_list_index_aux_Some f l : posbdd (lengthP l) f -> NoDup l ->
+  forall x, x ∈ l ->
+    is_Some (i ← list_index x l; l !! (f (Pos.of_succ_nat i):>nat)).
+Proof.
+  intros Hf Hl x Hx.
+  pose proof (lengthN_correct l).
+  apply elem_of_list_lookup in Hx as Hi.
+  destruct Hi as [i Hi].
+  apply list_index_Some_NoDup in Hi as Hi'; [|easy].
+  rewrite Hi'.
+  cbn.
+  apply lookup_lt_Some in Hi as Hilt.
+  apply lookup_lt_is_Some.
+  specialize (Hf (Pos.of_succ_nat i)).
+  lia.
+Qed.
+
+Lemma ppermute_alt_list_index f l : posbdd (lengthP l) f -> NoDup l ->
+  ppermute f l = omap (λ x, i ← list_index x l; l !! (f (Pos.of_succ_nat i):>nat)) l.
+Proof.
+  intros Hf Hl.
+  pose proof (lengthN_correct l).
+  specialize (ppermute_alt_list_index_aux_Some f l Hf Hl) as Hsome.
+  apply length_omap_all_is_Some in Hsome as Hlen.
+  apply (λ H, list_eq_same_length _ _ _ H eq_refl);
+  [now rewrite length_ppermute, Hlen|].
+  intros i x y.
+  rewrite length_ppermute.
+  intros Hi.
+  rewrite lookup_ppermute_alt_bdd by easy.
+  rewrite list_lookup_omap_all_is_Some by easy.
+  apply lookup_lt_is_Some in Hi as Hli.
+  destruct Hli as [li Hli].
+  rewrite Hli.
+  cbn.
+  apply list_index_Some_NoDup in Hli as Hli'; [|easy].
+  rewrite Hli'.
+  cbn.
+  congruence.
+Qed.
+
+Lemma ppermute_alt_list_index_total
+  f l : posbdd (lengthP l) f -> NoDup l ->
+  ppermute f l = (λ x, default x
+    (i ← list_index x l; l !! (f (Pos.of_succ_nat i):>nat))) <$> l.
+Proof.
+  intros Hf Hl.
+  rewrite ppermute_alt_list_index by easy.
+  now apply omap_all_is_Some_default, ppermute_alt_list_index_aux_Some.
+Qed.
+
+End list_index.
+
+Lemma graph_namedtensorlist_semantics_ppermute tg int_lab fi ext_lab :
+  NoDup int_lab -> length int_lab = num_internals tg ->
+  posperm (lengthP int_lab) fi ->
+  graph_namedtensorlist_semantics tg int_lab ext_lab =ntl=
+  graph_namedtensorlist_semantics tg (ppermute fi int_lab) ext_lab.
+Proof.
+  intros Hdup Hlen Hfi.
+  pose proof (lengthN_correct int_lab).
+  rewrite 2 graph_namedtensorlist_semantics_to_aux.
+  apply ntl_aeq_of_WF; [now rewrite <- graph_namedtensorlist_semantics_to_aux;
+    apply graph_namedtensorlist_semantics_WF|].
+
+
+  cbn.
+  rewrite (list_fmap_compose fst), fst_zip by now apply eq_reflexivity.
+  rewrite <- list_fmap_compose.
+  change (fst ∘ _) with (Pos.of_succ_nat).
+  rewrite (list_fmap_compose fst), fst_zip by
+    now rewrite length_ppermute; apply eq_reflexivity.
+  (* rewrite <- list_fmap_compose. *)
+  change (fst ∘ _) with (Pos.of_succ_nat).
+  pose proof (lengthN_correct int_lab).
+  exists (Pos.of_succ_nat
+      ∘ (λ x : Ty,
+           default x
+             (list_index x int_lab
+              ≫= λ i : Ty, int_lab !! (fi (Pos.of_succ_nat i):>nat)))
+      ∘ pos_to_nat_pred).
+  split_and!.
+  - intros _ _ (x & -> & Hx)%elem_of_list_to_set%elem_of_list_fmap
+      (y & -> & Hy)%elem_of_list_to_set%elem_of_list_fmap.
+    cbn.
+    rewrite 2 pos_to_nat_pred_of_nat.
+    apply elem_of_list_lookup in Hx as Hi.
+    apply elem_of_list_lookup in Hy as Hj.
+    destruct Hi as [i Hi], Hj as [j Hj].
+    apply list_index_Some_NoDup in Hi as Hi'; [|easy].
+    apply list_index_Some_NoDup in Hj as Hj'; [|easy].
+    rewrite Hi', Hj'.
+    cbn.
+    intros Heq%(inj Pos.of_succ_nat).
+    pose proof (posperm_bounded _ _ Hfi) as Hfibdd.
+    apply lookup_lt_Some in Hi as Hilt.
+    apply lookup_lt_Some in Hj as Hjlt.
+
+    assert (is_Some (int_lab !! (fi (Pos.of_succ_nat i) :> nat))) as Hfi_i. 1:{
+      apply lookup_lt_is_Some.
+      specialize (Hfibdd (Pos.of_succ_nat i)).
+      lia.
+    }
+    assert (is_Some (int_lab !! (fi (Pos.of_succ_nat j) :> nat))) as Hfi_j. 1:{
+      apply lookup_lt_is_Some.
+      specialize (Hfibdd (Pos.of_succ_nat j)).
+      lia.
+    }
+    destruct Hfi_i as [fii Hfii], Hfi_j as [fij Hfij].
+    rewrite Hfii, Hfij in Heq.
+    cbn in Heq.
+    subst fij.
+    specialize (NoDup_lookup _ _ _ _ Hdup Hfii Hfij)
+      as Heq%(inj pos_to_nat_pred).
+    apply (posperm_inj _ _ Hfi) in Heq as Heq%(inj _); [|lia..].
+    subst j.
+    congruence.
+  - rewrite ppermute_alt_list_index_total by now easy + apply posperm_bounded.
+    apply eq_reflexivity.
+    rewrite <- 2 list_fmap_compose.
+    apply list_fmap_ext; intros _ x Hx%elem_of_list_lookup_2.
+    cbn.
+    now rewrite pos_to_nat_pred_of_nat.
+  -
+    apply eq_reflexivity.
+    rewrite <- list_fmap_compose.
+    apply list_fmap_ext; intros _ k Hk%elem_of_list_lookup_2.
+    rewrite <- (elem_of_list_to_set (C:=gset nat)), <- dom_alt in Hk.
+    cbn [compose].
+    rewrite ppermute_alt_list_index_total by now easy + apply posperm_bounded.
+    rewrite zip_fmap_l, <- relabel_rels_mk_node.
+    reflexivity.
+Qed.
+
+Lemma NoDup_fmap_ind `(f : A -> B) (P : list A -> Prop)
+  (Pnil : P []) (Pcons : forall a l, f a ∉ f <$> l -> NoDup (f <$> l) ->
+    P l -> P (a :: l)) : forall l, NoDup (f <$> l) -> P l.
+Proof.
+  intros l.
+  induction l; [easy|].
+  cbn; rewrite NoDup_cons.
+  intros []; eauto.
+Qed.
+
+Lemma input_edges_ext_label_irrel lint lext lext' k :
+  lext.*2 = lext'.*2 ->
+  input_edges lint lext k = input_edges lint lext' k.
+Proof.
+  intros Hlext.
+  unfold input_edges; f_equal.
+  unfold node_input_edges.
+  rewrite 2 (list_fmap_compose snd), <- 2 list_filter_fmap.
+  now rewrite Hlext.
+Qed.
+
+Lemma output_edges_ext_label_irrel lint lext lext' k :
+  lext.*2 = lext'.*2 ->
+  output_edges lint lext k = output_edges lint lext' k.
+Proof.
+  intros Hlext.
+  unfold output_edges; f_equal.
+  unfold node_output_edges.
+  rewrite 2 (list_fmap_compose snd (_ ∘ snd)), <- 2 list_filter_fmap.
+  now rewrite Hlext.
+Qed.
+
+Lemma mk_node_ext_label_irrel lint lext lext' k :
+  lext.*2 = lext'.*2 ->
+  mk_node lint lext k = mk_node lint lext' k.
+Proof.
+  intros Hext.
+  unfold mk_node.
+  f_equal; [f_equal|];
+  [now apply input_edges_ext_label_irrel|
+   now apply output_edges_ext_label_irrel].
+Qed.
+
+Lemma zip_with_irrel_l {A B C} (f : B -> C) (l l' : list A) (k : list B) :
+  length l = length l' ->
+  zip_with (λ _ b, f b) l k = zip_with (λ _ b, f b) l' k.
+Proof.
+  intros Hall%Forall2_same_length.
+  revert k;
+  induction Hall; intros []; cbn; congruence.
+Qed.
+
+Lemma zip_with_irrel_r {A B C} (f : A -> C) (l : list A) (k k' : list B) :
+  length k = length k' ->
+  zip_with (λ a _, f a) l k = zip_with (λ a _, f a) l k'.
+Proof.
+  intros Hall%Forall2_same_length.
+  revert l;
+  induction Hall; intros []; cbn; congruence.
+Qed.
+
+Lemma graph_namedtensorlist_semantics_ext_lab_irrel tg int_lab ext_lab ext_lab' :
+  length ext_lab = length ext_lab' ->
+  graph_namedtensorlist_semantics tg int_lab ext_lab =
+  graph_namedtensorlist_semantics tg int_lab ext_lab'.
+Proof.
+  intros Hlen.
+  unfold graph_namedtensorlist_semantics.
+  f_equal.
+  apply list_fmap_ext; intros _ x _.
+  apply mk_node_ext_label_irrel.
+  rewrite 2 fmap_zip_with; cbn.
+  now apply zip_with_irrel_l.
+Qed.
+
+
+
+Lemma graph_namedtensorlist_semantics_perm_eq tg int_lab int_lab'
+  ext_lab ext_lab' :
+  NoDup int_lab -> length int_lab = num_internals tg ->
+  int_lab ≡ₚ int_lab' ->
+  length ext_lab = length ext_lab' ->
+  graph_namedtensorlist_semantics tg int_lab ext_lab =ntl=
+  graph_namedtensorlist_semantics tg int_lab' ext_lab'.
+Proof.
+  intros Hdup Hlen (f & Hf & <- & Hlook)%perm_exists_posperm Hext.
+  etransitivity; [apply graph_namedtensorlist_semantics_ppermute; eauto|].
+  apply eq_reflexivity.
+  now apply graph_namedtensorlist_semantics_ext_lab_irrel.
+Qed.
+
+
+Lemma graph_namedtensorlist_semantics_seq_correct' tg :
+  graph_tensorlist_semantics tg =
+  ntl2tl (graph_namedtensorlist_semantics tg (seq 0 (num_internals tg))
+	  (seq 0 (num_externals tg))).
+Proof.
+  rewrite graph_namedtensorlist_semantics_seq_correct.
+  now rewrite tl2ntl2tl.
+Qed.
+
+Lemma internal_edges_perm ns es es' :
+  es ≡ₚ es' ->
+  @internal_edges T (mk_tg ns es) ≡ₚ internal_edges (mk_tg ns es').
+Proof.
+  intros Hes.
+  unfold internal_edges; cbn.
+  now f_equiv.
+Qed.
+
+Lemma external_edges_perm ns es es' :
+  es ≡ₚ es' ->
+  @external_edges T (mk_tg ns es) ≡ₚ external_edges (mk_tg ns es').
+Proof.
+  intros Hes.
+  unfold external_edges; cbn.
+  now f_equiv.
+Qed.
+
+
+Lemma graph_tensorlist_semantics_perm_eq_pairs_elab ns es es' :
+  es ≡ₚ es' ->
+  exists idxs idxs',
+  idxs ≡ₚ seq 0 (num_internals (mk_tg ns es)) /\
+  idxs' ≡ₚ seq 0 (num_externals (mk_tg ns es)) /\
+  tl2ntl (graph_tensorlist_semantics (mk_tg ns es)) ≡ntl'≡ₚ
+  graph_namedtensorlist_semantics_aux
+    (zip idxs (internal_edges (mk_tg ns es')))
+    (zip idxs' (external_edges (mk_tg ns es')))
+    (map_to_list ns).*1 /\
+  graph_namedtensorlist_semantics_aux
+    (zip idxs (internal_edges (mk_tg ns es')))
+    (zip idxs' (external_edges (mk_tg ns es')))
+    (map_to_list ns).*1
+    =ntl= tl2ntl (graph_tensorlist_semantics (mk_tg ns es')).
+Proof.
+  intros Hes.
+  apply (internal_edges_perm ns) in Hes as Hies.
+  apply (external_edges_perm ns) in Hes as Hees.
+
+  apply perm_exists_perm_seq in Hies as Hidxs.
+  apply perm_exists_perm_seq in Hees as Hidxs'.
+
+  destruct Hidxs as (idxs & Hidxs & Himap).
+  destruct Hidxs' as (idxs' & Hidxs' & Himap').
+  exists idxs, idxs'.
+  split; [easy|].
+  split; [easy|].
+  split.
+  - rewrite <- graph_namedtensorlist_semantics_seq_correct.
+    rewrite graph_namedtensorlist_semantics_to_aux.
+    cbn [nodes].
+    eapply graph_namedtensorlist_semantics_aux_perm_eq';
+    [rewrite fst_zip by (now rewrite length_seq);
+     apply NoDup_seq|..|reflexivity].
+    + etransitivity; [|apply Himap].
+      now rewrite imap_to_zip_with_seq.
+    + etransitivity; [|apply Himap'].
+      now rewrite imap_to_zip_with_seq.
+  - rewrite <- graph_namedtensorlist_semantics_to_aux.
+    rewrite <- graph_namedtensorlist_semantics_seq_correct.
+    apply graph_namedtensorlist_semantics_perm_eq.
+    + rewrite Hidxs; apply NoDup_seq.
+    + rewrite Hidxs.
+      now rewrite length_seq, Hies.
+    + rewrite Hidxs.
+      f_equiv.
+      now rewrite Hies.
+    + rewrite Hidxs'.
+      now rewrite 2 length_seq, Hees.
+Qed.
+
+
+Lemma graph_tensorlist_semantics_perm_eq_pairs ns es es' :
+  es ≡ₚ es' ->
+  exists mid,
+  tl2ntl (graph_tensorlist_semantics (mk_tg ns es)) ≡ntl'≡ₚ mid /\
+  mid =ntl= tl2ntl (graph_tensorlist_semantics (mk_tg ns es')).
+Proof.
+  intros Hes.
+  apply (graph_tensorlist_semantics_perm_eq_pairs_elab ns) in Hes.
+  naive_solver.
+Qed.
+
+
+
+
 
 End TensorGraphExpr.
